4a done, starting to work on tokeneer project

Sorting/sorting.dfy
@@ -4,7 +4,6 @@ class Sorted {
 //------------- 1a -------------
 
 //solution 1
-
 predicate Sorted( a: seq<int>)
 	requires a != null;
 
@@ -13,27 +12,22 @@ reads a;
  forall i : int :: 0 <= i < a.Length-1 ==> a[i] < a[i+1]
 }
 
-
-
 // ------------- 1b -------------
 
 // solution 2
-
 predicate Sorted2(a : seq<int>)
 	requires a != null;
 
 reads a;
 {
-
 forall i , j : int :: 0 <= i < j < a.Length ==> a[i]< a[j]
-
 }
 
 
 
 // -------------   2a   -------------
 /*
-ghost method Sortedlol(a : seq<int>)
+method SortedGhost(a : seq<int>)
 	requires a != null;
 	requires a.Length >= 2;
 
@@ -41,38 +35,74 @@ ghost method Sortedlol(a : seq<int>)
 {
 }
 */
-ghost method Sortedlol2(a : seq<int>)
+
+ method Sortedlghost2(a : seq<int>)
 
 	requires a != null;
 	requires  a.Length >= 2;
   	ensures Sorted2(a) ==> Sorted(a)
 {
+
 }
 
 
-// -------------   2b   ------------- PAPER
+// -------------   2b   ------PAPER
 
 
 // -------------   3a   -------------
-
 /*
 
 With multiset we get that the sequence [cow, horse, cow, horse] is equivalent to
 the sequence [horse , cow, horse, cow].
 
 the sequence and repetitions of the sequence does not matter, it is just the 
-elements that are in the multiset.
+elements that are in the multiset and the occuances of it.
 
 
 So what p checks is if the number of different animals in multiset a is 
 the same as in multiset b
-
-
-
-
-
-FOR 3B, THINK ABOUT BUTTERFLIES EXISTS IN B IN A, EXISTS PREDICATE ETC 
 */
+
+predicate p(a :seq<int> , b : seq<int>)
+{
+|a| == |b| && forall i : int :: 0 <= i < a.Length ==>  helper(a,a[i],0) == helper(b,b[i],0)
+}
+
+function helper (s : seq<int>,value : int, counter : int) : int{
+
+if (s == []) then counter 
+else if (s[0] == value) then helper(s[1..],value,counter+1) 
+else  helper(s[1..],value,counter)
+
+}
+
+//---------------- 4a ----------------------
+
+method sortme(src : arr<int>) 
+requires src != null
+ensures 	p(t[..]) &&
+			(old(src) == src)   // sorted in place, ref to array should be the same
+{   }
+
+
+//----------------- 4b ---------------------
+
+/*
+It's a bit unclear what you want from us, do you want a method or 
+*/
+
+
+
+
+
+
+
+
+
+
+
+
+
 
 
 
