tokeneer/idStation.dfy
@@ -1,0 +1,16 @@
+
+/*
+class ID station, checks whether the user 
+
+
+*/
+
+class IDStation{
+
+
+var securityDoor : bool;
+
+
+
+
+}
