tokeneer/token.dfy
@@ -1,0 +1,13 @@
+/*
+A token class, the security level is represented 
+[(low by 1), (medium by 2), (high by 3)]
+
+*/
+
+class Token {
+	var security_level : int;
+	var fingerPrint : int;
+
+
+}
+
